keyset_ra.v
@@ -1,11 +1,14 @@
-Add LoadPath "/home/nisarg/Academics/templates".
 From iris.algebra Require Import gset.
 From iris.proofmode Require Import tactics.
 Set Default Proof Using "All".
 Require Export flows.
 
+Section keyset_ra.
+
+Context `{Countable K}.
+
 Inductive prodT := 
-  prod : gset key*gset key → prodT
+  prod : gset K*gset K → prodT
 | prodTop : prodT
 | prodBot : prodT.
 
@@ -51,7 +54,7 @@ Proof.
     destruct (decide (g ∪ g1 ## g3)). destruct (decide (g0 ∪ g2 ## g4)). apply leibniz_equiv_iff.
     assert (g ∪ (g1 ∪ g3) = g ∪ g1 ∪ g3). { set_solver. }
     assert (g0 ∪ (g2 ∪ g4) = g0 ∪ g2 ∪ g4). { set_solver. }
-    rewrite H. rewrite H0. reflexivity.
+    rewrite H0. rewrite H1. reflexivity.
     unfold not in n. exfalso. apply n. set_solver.
     unfold not in n. exfalso. apply n. set_solver.
     unfold not in n. exfalso. apply n. set_solver.
@@ -107,9 +110,9 @@ Proof.
     destruct y. destruct p. unfold op, prodOp. done. unfold op, prodOp. done. unfold op, prodOp. done.
 Qed.
 
-Canonical Structure keysetRA := discreteR prodT prodRA_mixin.
+Canonical Structure KsetRA := discreteR prodT prodRA_mixin.
 
-Instance prodRA_cmra_discrete : CmraDiscrete keysetRA.
+Instance prodRA_cmra_discrete : CmraDiscrete KsetRA.
 Proof. apply discrete_cmra_discrete. Qed.
 
 Lemma prod_ucmra_mixin : UcmraMixin prodT.
@@ -120,22 +123,22 @@ Qed.
     
 Canonical Structure keysetUR : ucmraT := UcmraT prodT prod_ucmra_mixin.
 
-Parameter KS : gset key.                                
+Parameter KS : gset K.                                
 
-Lemma auth_ks_included (a1 a2 b1 b2: gset key) : 
+Lemma auth_ks_included (a1 a2 b1 b2: gset K) : 
            ✓ prod (a1, b1) → ✓ prod (a2, b2) → prod (a1, b1) ≼ prod (a2, b2) 
               → (a1 = a2 ∧ b1 = b2) ∨ 
                   (∃ a0 b0, a2 = a1 ∪ a0 ∧ b2 = b1 ∪ b0 ∧ a1 ## a0 ∧ b1 ## b0 ∧ b1 ⊆ a1 ∧ b2 ⊆ a2 ∧ b0 ⊆ a0).
 Proof.
-  intros H1 H2 H. destruct H as [z H]. assert (✓ z). { apply (cmra_valid_op_r (prod (a1, b1))).
-  rewrite <-H. done. } rewrite /(✓ prod (a1, b1)) /= in H1. rewrite /(✓ prod (a2, b2)) /= in H2.
+  intros H1 H2 H0. destruct H0 as [z H0]. assert (✓ z). { apply (cmra_valid_op_r (prod (a1, b1))).
+  rewrite <- H0. done. } rewrite /(✓ prod (a1, b1)) /= in H1. rewrite /(✓ prod (a2, b2)) /= in H2.
   destruct z.
-  - destruct p. rewrite /(✓ prod (g, g0)) /= in H0. rewrite /(⋅) /= in H.
+  - destruct p. rewrite /(✓ prod (g, g0)) /= in H3. rewrite /(⋅) /= in H0.
     destruct (decide (b1 ⊆ a1)). destruct (decide (g0 ⊆ g)). destruct (decide (a1 ## g)).
-    destruct (decide (b1 ## g0)). right. exists g, g0. set_solver. inversion H. inversion H.
-    inversion H. inversion H.
+    destruct (decide (b1 ## g0)). right. exists g, g0. set_solver. inversion H0. inversion H0.
+    inversion H0. inversion H0.
   - rewrite /(✓ prodTop) /= in H0. exfalso. done.
-  - rewrite /(⋅) /= in H. inversion H. left. done.
+  - rewrite /(⋅) /= in H0. inversion H0. left. done.
 Qed.  
 
 Lemma auth_ks_local_update_insert K1 C Cn k:
@@ -144,22 +147,22 @@ Lemma auth_ks_local_update_insert K1 C Cn k:
 Proof.
   intros [H1 [H2 [H3 [H4 HKS]]]]. apply local_update_discrete. intros z.
   intros _. intros. split. rewrite /(✓ prod (KS, C ∪ {[k]})) /=. 
-  rewrite /(cmra_valid keysetRA) /=. rewrite /(✓ prod (KS, C)) /= in H1.
-  set_solver. rewrite /(opM) /= in H.
-  destruct z. rewrite /(opM) /=. destruct c. destruct p. rewrite /(op) /= in H.
-  rewrite /(cmra_op keysetRA) /= in H. destruct (decide (Cn ⊆ K1)).
+  rewrite /(cmra_valid KsetRA) /=. rewrite /(✓ prod (KS, C)) /= in H1.
+  set_solver. rewrite /(opM) /= in H0.
+  destruct z. rewrite /(opM) /=. destruct c. destruct p. rewrite /(op) /= in H0.
+  rewrite /(cmra_op KsetRA) /= in H0. destruct (decide (Cn ⊆ K1)).
   destruct (decide (g0 ⊆ g)). destruct (decide (K1 ## g)). destruct (decide (Cn ## g0)).
-  inversion H. rewrite /(op) /=. rewrite /(cmra_op keysetRA) /=. destruct (decide (Cn ∪ {[k]} ⊆ K1)).
+  inversion H0. rewrite /(op) /=. rewrite /(cmra_op KsetRA) /=. destruct (decide (Cn ∪ {[k]} ⊆ K1)).
   destruct (decide (g0 ⊆ g)). destruct (decide (K1 ## g)). destruct (decide (Cn ∪ {[k]} ## g0)).
-  assert (Cn ∪ g0 ∪ {[k]} = Cn ∪ {[k]} ∪ g0). { set_solver. } rewrite H0. rewrite H5. done.
+  assert (Cn ∪ g0 ∪ {[k]} = Cn ∪ {[k]} ∪ g0). { set_solver. } rewrite H6. rewrite H5. done.
   unfold not in n. exfalso. apply n. set_solver. unfold not in n. exfalso. apply n. set_solver.
   unfold not in n. exfalso. apply n. set_solver. unfold not in n. exfalso. apply n. set_solver.
   unfold not in n. exfalso. apply n. set_solver. unfold not in n. exfalso. apply n. set_solver.
   unfold not in n. exfalso. apply n. set_solver. unfold not in n. exfalso. apply n. set_solver.
-  rewrite /(op) /= in H. rewrite /(cmra_op keysetRA) /= in H. inversion H.
-  rewrite /(op) /= in H. rewrite /(cmra_op keysetRA) /= in H. inversion H.
-  rewrite /(op) /=. rewrite /(cmra_op keysetRA) /=. done.
-  rewrite /(opM) /=. inversion H. done.
+  rewrite /(op) /= in H0. rewrite /(cmra_op KsetRA) /= in H0. inversion H0.
+  rewrite /(op) /= in H0. rewrite /(cmra_op KsetRA) /= in H0. inversion H0.
+  rewrite /(op) /=. rewrite /(cmra_op KsetRA) /=. done.
+  rewrite /(opM) /=. inversion H0. done.
 Qed.
 
 Lemma auth_ks_local_update_delete K1 C Cn k:
@@ -168,23 +171,26 @@ Lemma auth_ks_local_update_delete K1 C Cn k:
 Proof.
   intros [H1 [H2 [H3 H4]]]. apply local_update_discrete. intros z.
   intros _. intros. split. rewrite /(✓ prod (KS, C ∖ {[k]})) /=. 
-  rewrite /(cmra_valid keysetRA) /=. rewrite /(✓ prod (KS, C)) /= in H1.
-  set_solver. rewrite /(opM) /= in H.
-  destruct z. rewrite /(opM) /=. destruct c. destruct p. rewrite /(op) /= in H.
-  rewrite /(cmra_op keysetRA) /= in H. destruct (decide (Cn ⊆ K1)).
+  rewrite /(cmra_valid KsetRA) /=. rewrite /(✓ prod (KS, C)) /= in H1.
+  set_solver. rewrite /(opM) /= in H0.
+  destruct z. rewrite /(opM) /=. destruct c. destruct p. rewrite /(op) /= in H0.
+  rewrite /(cmra_op KsetRA) /= in H0. destruct (decide (Cn ⊆ K1)).
   destruct (decide (g0 ⊆ g)). destruct (decide (K1 ## g)). destruct (decide (Cn ## g0)).
-  inversion H. rewrite /(op) /=. rewrite /(cmra_op keysetRA) /=. destruct (decide (Cn ∖ {[k]} ⊆ K1)).
+  inversion H. rewrite /(op) /=. rewrite /(cmra_op KsetRA) /=. destruct (decide (Cn ∖ {[k]} ⊆ K1)).
   destruct (decide (g0 ⊆ g)). destruct (decide (K1 ## g)). destruct (decide (Cn ∖ {[k]} ## g0)).
   assert (k ∉ g0). { set_solver. }
-  assert ((Cn ∪ g0) ∖ {[k]} = Cn ∖ {[k]} ∪ g0). { set_solver. } rewrite H7. rewrite H5. done.
+  assert ((Cn ∪ g0) ∖ {[k]} = Cn ∖ {[k]} ∪ g0). { set_solver. } rewrite <- H6. inversion H0. done.
   unfold not in n. exfalso. apply n. set_solver. unfold not in n. exfalso. apply n. set_solver.
   unfold not in n. exfalso. apply n. set_solver. unfold not in n. exfalso. apply n. set_solver.
   unfold not in n. exfalso. apply n. set_solver. unfold not in n. exfalso. apply n. set_solver.
   unfold not in n. exfalso. apply n. set_solver. unfold not in n. exfalso. apply n. set_solver.
-  rewrite /(op) /= in H. rewrite /(cmra_op keysetRA) /= in H. inversion H.
-  rewrite /(op) /= in H. rewrite /(cmra_op keysetRA) /= in H. inversion H.
-  rewrite /(op) /=. rewrite /(cmra_op keysetRA) /=. done.
-  rewrite /(opM) /=. inversion H. done.
+  rewrite /(op) /= in H0. rewrite /(cmra_op KsetRA) /= in H0. inversion H0.
+  rewrite /(op) /= in H0. rewrite /(cmra_op KsetRA) /= in H0. inversion H0.
+  rewrite /(op) /=. rewrite /(cmra_op KsetRA) /=. done.
+  rewrite /(opM) /=. inversion H0. done.
 Qed.
 
 
+End keyset_ra.
+
+Arguments keysetUR _ {_ _}.
